Test/civl/pending-async-noninterference-fail.bpl
@@ -6,8 +6,8 @@ var {:layer 0,1} x:int;
 procedure {:yield_invariant} {:layer 1} yield_x(n: int);
 requires x >= n;
 
-type {:pending_async}{:datatype} PA;
-function {:constructor} A() : PA;
+datatype {:pending_async} PA { A() }
+
 
 function {:inline} NoPAs () : [PA]int
 { (lambda pa:PA :: 0) }
