Test/monomorphize/finite-inst-error1.bpl
@@ -1,10 +1,6 @@
-// RUN: %parallel-boogie /monomorphize "%s" > "%t"
+// RUN: %parallel-boogie /lib:base /monomorphize "%s" > "%t"
 // RUN: %diff "%s.expect" "%t"
 // test for use of cycle of increasing types
-
-type {:datatype} Option _;
-function {:constructor} None<T>(): Option T;
-function {:constructor} Some<T>(t: T): Option T;
 
 procedure A<T>(i: T)
 {
